ok

SStructTT/Dynamic/Typed.lean
@@ -11,44 +11,44 @@ inductive Typed : Static.Ctx Srt -> Dynamic.Ctx Srt -> Tm Srt -> Tm Srt -> Prop 
     Has Δ x s A ->
     Typed Γ Δ (.var x) A
 
-  | lam_im {Γ Δ A B m} s {sA iA} :
+  | lam_im {Γ Δ A B m s sA iA} :
     Δ !≤ s ->
     Γ ⊢ A : .srt sA iA ->
     Typed (A :: Γ) (_: Δ) m B ->
     Typed Γ Δ (.lam A m .im s) (.pi A B .im s)
 
-  | lam_ex {Γ Δ Δ1 A B m} s {sA iA} :
+  | lam_ex {Γ Δ Δ1 A B m s sA iA} :
     Δ !≤ s ->
     Γ ⊢ A : .srt sA iA ->
     Ext A sA Δ Δ1 ->
     Typed (A :: Γ) Δ1 m B ->
     Typed Γ Δ (.lam A m .ex s) (.pi A B .ex s)
 
-  | app_im Γ Δ A B m n s :
+  | app_im {Γ Δ A B m n s} :
     Typed Γ Δ m (.pi A B .im s) ->
     Γ ⊢ n : A ->
     Typed Γ Δ (.app m n .im) B.[n/]
 
-  | app_ex Γ Δ1 Δ2 Δ A B m n s :
+  | app_ex {Γ Δ1 Δ2 Δ A B m n s} :
     Merge Δ1 Δ2 Δ ->
     Typed Γ Δ1 m (.pi A B .ex s) ->
     Typed Γ Δ2 n A ->
     Typed Γ Δ (.app m n .ex) B.[n/]
 
-  | tup_im Γ Δ A B m n s i :
+  | tup_im {Γ Δ A B m n s i} :
     Γ ⊢ .sig A B .im s : .srt s i ->
     Typed Γ Δ m A ->
     Γ ⊢ n : B.[m/] ->
     Typed Γ Δ (.tup m n .im s) (.sig A B .im s)
 
-  | tup_ex Γ Δ1 Δ2 Δ A B m n s i :
+  | tup_ex {Γ Δ1 Δ2 Δ A B m n s i} :
     Merge Δ1 Δ2 Δ ->
     Γ ⊢ .sig A B .ex s : .srt s i ->
     Typed Γ Δ1 m A ->
     Typed Γ Δ2 n B.[m/] ->
     Typed Γ Δ (.tup m n .ex s) (.sig A B .ex s)
 
-  | proj_im Γ Δ1 Δ2 Δ3 Δ A B C m n s sA sC iC :
+  | proj_im {Γ Δ1 Δ2 Δ3 Δ A B C m n s sA sC iC} :
     Merge Δ1 Δ2 Δ ->
     .sig A B .im s :: Γ ⊢ C : .srt sC iC ->
     Typed Γ Δ1 m (.sig A B .im s) ->
@@ -56,7 +56,7 @@ inductive Typed : Static.Ctx Srt -> Dynamic.Ctx Srt -> Tm Srt -> Tm Srt -> Prop 
     Typed (B :: A :: Γ) (_: Δ3) n C.[.tup (.var 1) (.var 0) .im s .: shift 2] ->
     Typed Γ Δ (.proj C m n .im) C.[m/]
 
-  | proj_ex Γ Δ1 Δ2 Δ3 Δ4 Δ A B C m n s sA sB sC iC :
+  | proj_ex {Γ Δ1 Δ2 Δ3 Δ4 Δ A B C m n s sA sB sC iC} :
     Merge Δ1 Δ2 Δ ->
     .sig A B .ex s :: Γ ⊢ C : .srt sC iC ->
     Typed Γ Δ1 m (.sig A B .ex s) ->
@@ -65,17 +65,17 @@ inductive Typed : Static.Ctx Srt -> Dynamic.Ctx Srt -> Tm Srt -> Tm Srt -> Prop 
     Typed (B :: A :: Γ) Δ4 n C.[.tup (.var 1) (.var 0) .ex s .: shift 2] ->
     Typed Γ Δ (.proj C m n .ex) C.[m/]
 
-  | tt Γ Δ :
+  | tt {Γ Δ} :
     Wf Γ Δ ->
     Δ.Forall (fun e => e = none) ->
     Typed Γ Δ .tt .bool
 
-  | ff Γ Δ :
+  | ff {Γ Δ} :
     Wf Γ Δ ->
     Δ.Forall (fun e => e = none) ->
     Typed Γ Δ .ff .bool
 
-  | ite Γ Δ1 Δ2 Δ A m n1 n2 s i :
+  | ite {Γ Δ1 Δ2 Δ A m n1 n2 s i} :
     Merge Δ1 Δ2 Δ ->
     (.bool :: Γ) ⊢ A : .srt s i ->
     Typed Γ Δ1 m .bool ->
@@ -89,7 +89,7 @@ inductive Typed : Static.Ctx Srt -> Dynamic.Ctx Srt -> Tm Srt -> Tm Srt -> Prop 
     Γ ⊢ n : .idn B a b ->
     Typed Γ Δ (.rw A m n) A.[n,b/]
 
-  | conv Γ Δ A B m s i :
+  | conv {Γ Δ A B m s i} :
     A === B ->
     Typed Γ Δ m A ->
     Γ ⊢ B : .srt s i ->
@@ -97,11 +97,11 @@ inductive Typed : Static.Ctx Srt -> Dynamic.Ctx Srt -> Tm Srt -> Tm Srt -> Prop 
 
 inductive Wf : Static.Ctx Srt -> Dynamic.Ctx Srt -> Prop where
   | nil : Wf [] []
-  | ex Γ Δ A s i :
+  | ex {Γ Δ A s i} :
     Γ ⊢ A : .srt s i ->
     Wf Γ Δ ->
     Wf (A :: Γ) (A :⟨s⟩ Δ)
-  | im Γ Δ A s i :
+  | im {Γ Δ A s i} :
     Γ ⊢ A : .srt s i ->
     Wf Γ Δ ->
     Wf (A :: Γ) (_: Δ)
@@ -109,3 +109,121 @@ end
 
 notation:50 Γ:50 "; " Δ:51 " ⊢ " m:51 " : " A:51 => Typed Γ Δ m A
 notation:50 Γ:50 "; " Δ:51 " ⊢ " => Wf Γ Δ
+
+-- Register non-mutual recursor as default.
+@[induction_eliminator]
+def Typed.rec_non_mutual {motive : ∀ Γ Δ m a, @Typed Srt _ Γ Δ m a -> Prop} :=
+  Typed.rec (motive_1 := motive) (motive_2 := fun _ _ _ => True)
+
+-- Register non-mutual recursor as default.
+@[induction_eliminator]
+def Wf.rec_non_mutual {motive : ∀ Γ Δ, @Wf Srt _ Γ Δ -> Prop} :=
+  Wf.rec (motive_1 := fun _ _ _ _ _ => True) (motive_2 := motive)
+
+lemma Wf.size {Γ : Static.Ctx Srt} {Δ : Dynamic.Ctx Srt} :
+    Γ ; Δ ⊢ -> Γ.length = Δ.length := by
+  intro wf
+  induction wf
+  all_goals aesop
+
+lemma Wf.merge {Γ : Static.Ctx Srt} {Δ Δ1 Δ2 : Dynamic.Ctx Srt} :
+    Merge Δ1 Δ2 Δ -> Γ ; Δ1 ⊢ -> Γ ; Δ2 ⊢ -> Γ ; Δ ⊢ := by
+  intro mrg wf1
+  induction mrg generalizing Γ
+  case nil =>
+    cases wf1
+    aesop
+  case contra ih =>
+    intro wf2
+    cases wf1
+    cases wf2
+    aesop (add safe Wf)
+  case left ih =>
+    intro wf2
+    cases wf1
+    cases wf2
+    aesop (add safe Wf)
+  case right ih =>
+    intro wf2
+    cases wf1
+    cases wf2
+    aesop (add safe Wf)
+  case im ih =>
+    intro wf2
+    cases wf1
+    cases wf2
+    aesop (add safe Wf)
+
+lemma Wf.split {Γ : Static.Ctx Srt} {Δ Δ1 Δ2 : Dynamic.Ctx Srt} :
+    Merge Δ1 Δ2 Δ -> Γ ; Δ ⊢ -> Γ ; Δ1 ⊢ ∧ Γ ; Δ2 ⊢ := by
+  intro mrg wf
+  induction mrg generalizing Γ
+  case nil =>
+    cases wf
+    aesop (add safe Wf)
+  case contra ih =>
+    cases wf
+    aesop (add safe Wf)
+  case left ih =>
+    cases wf
+    aesop (add safe Wf)
+  case right ih =>
+    cases wf
+    aesop (add safe Wf)
+  case im ih =>
+    cases wf
+    aesop (add safe Wf)
+
+lemma Typed.toWf {Γ : Static.Ctx Srt} {Δ : Dynamic.Ctx Srt} {A m} :
+    Γ ; Δ ⊢ m : A -> Γ ; Δ ⊢ := by
+  intro ty
+  induction ty <;> try (solve | aesop)
+  case lam_im ih =>
+    cases ih
+    aesop
+  case lam_ex ih =>
+    cases ih
+    case ex ext _ =>
+      cases ext
+      assumption
+    case im ext _ =>
+      cases ext
+      assumption
+  case app_ex mrg _ _ ih1 ih2 =>
+    apply Wf.merge mrg ih1 ih2
+  case tup_ex mrg _ _ _ ih1 ih2 =>
+    apply Wf.merge mrg ih1 ih2
+  case proj_im mrg _ _ ext _ ih1 ih2 =>
+    cases ext with
+    | ex =>
+      rcases ih2 with _ | _ | ⟨_, ih2⟩
+      rcases ih2 with _ | ⟨_, ih2⟩
+      apply Wf.merge mrg ih1 ih2
+    | wk =>
+      rcases ih2 with _ | _ | ⟨_, ih2⟩
+      rcases ih2 with _ | _ | ⟨_, ih2⟩
+      apply Wf.merge mrg ih1 ih2
+  case proj_ex mrg _ _ ext1 ext2 _ ih1 ih2 =>
+    cases ext1 with
+    | ex =>
+      cases ext2 with
+      | ex =>
+        rcases ih2 with _ | ⟨_, ih2⟩
+        rcases ih2 with _ | ⟨_, ih2⟩
+        apply Wf.merge mrg ih1 ih2
+      | wk =>
+        rcases ih2 with _ | _ | ⟨_, ih2⟩
+        rcases ih2 with _ | ⟨_, ih2⟩
+        apply Wf.merge mrg ih1 ih2
+    | wk =>
+      cases ext2 with
+      | ex =>
+        rcases ih2 with _ | ⟨_, ih2⟩
+        rcases ih2 with _ | _ | ⟨_, ih2⟩
+        apply Wf.merge mrg ih1 ih2
+      | wk =>
+        rcases ih2 with _ | _ | ⟨_, ih2⟩
+        rcases ih2 with _ | _ | ⟨_, ih2⟩
+        apply Wf.merge mrg ih1 ih2
+  case ite mrg _ _ _ _ ih1 ih2 _ =>
+    apply Wf.merge mrg ih1 ih2
