SStructTT.lean
@@ -18,3 +18,4 @@ import SStructTT.Static.Progress
 
 import SStructTT.Dynamic.Context
 import SStructTT.Dynamic.Typed
+import SStructTT.Dynamic.Renaming
