SStructTT/Dynamic/Renaming.lean
@@ -1,0 +1,28 @@
+import SStructTT.Dynamic.Typed
+
+namespace Dynamic
+variable {Srt : Type} [inst : SStruct Srt]
+
+@[aesop safe (rule_sets := [rename]) [constructors]]
+inductive AgreeRen : (Var -> Var) ->
+  Static.Ctx Srt -> Dynamic.Ctx Srt ->
+  Static.Ctx Srt -> Dynamic.Ctx Srt -> Prop
+where
+  | nil {ξ} :
+    AgreeRen ξ [] [] [] []
+  | ex {Γ Γ' Δ Δ' A s i ξ} :
+    Γ ⊢ A : .srt s i ->
+    AgreeRen ξ Γ Δ Γ' Δ' ->
+    AgreeRen (upren ξ)
+      (A :: Γ) (A :⟨s⟩ Δ) (A.[ren ξ] :: Γ') (A.[ren ξ] :⟨s⟩ Δ')
+  | im {Γ Γ' Δ Δ' A s i ξ} :
+    Γ ⊢ A : .srt s i ->
+    AgreeRen ξ Γ Δ Γ' Δ' ->
+    AgreeRen (upren ξ)
+      (A :: Γ) (_: Δ) (A.[ren ξ] :: Γ') (_: Δ')
+  | wk {Γ Γ' Δ Δ' A s i ξ} :
+    Γ' ⊢ A : .srt s i ->
+    AgreeRen ξ Γ Δ Γ' Δ' ->
+    AgreeRen (ξ !>> (.+1)) Γ Δ (A :: Γ') (_: Δ')
+
+-- lemma AgreeRen.toStatic
